thys/Substitution/Codata.thy
@@ -12,26 +12,6 @@ theory Codata
   imports Codata_Customization
 begin
 
-interpretation Expression_with_Birecursor Eperm EVrs "card_suc Gbd" Ector
-proof (standard, safe)
-  fix Pvalid :: "'p \<Rightarrow> bool"
-  and Pperm :: "('a \<Rightarrow> 'a) \<Rightarrow> 'p \<Rightarrow> 'p"
-  and PVrs :: "'p \<Rightarrow> 'a set"
-  and Ector' :: "('a, 'a, 'p \<Rightarrow> 'a E, 'p \<Rightarrow> 'a E) G \<Rightarrow> 'p \<Rightarrow> 'a E"
-  assume "Bimodel Pvalid Pperm PVrs Eperm EVrs (card_suc Gbd) Ector Ector'"
-  (* interpret corec: COREC  *)
-  (* term corec.COREC *)
-  show "\<exists>rec. (\<forall>u p. Pvalid p \<and> noclashE u \<and> GVrs2 u \<inter> PVrs p = {} \<longrightarrow> 
-    rec (Ector u) p = Ector' (Gmap rec rec u) p) \<and>
-    (\<forall>e p \<sigma>. bij \<sigma> \<longrightarrow> |supp \<sigma>| <o |UNIV| \<longrightarrow> Pvalid p \<longrightarrow> rec (Eperm \<sigma> e) p = Eperm \<sigma> (rec e (Pperm (inv \<sigma>) p))) \<and>
-    (\<forall>e p. Pvalid p \<longrightarrow> EVrs (rec e p) \<subseteq> PVrs p \<union> EVrs e)"
-    sorry
-qed
-
-interpretation birec_codata: Expression_with_Birecursor_for_Subst_Strong Eperm EVrs "card_suc Gbd" Ector
-  by standard
-
-print_statement birec_codata.Esub_Strong.E_pbmv_axioms
 
 abbreviation "IMSUPP \<delta> \<rho> \<rho>' \<equiv> imsupp \<delta> \<union> IImsupp' (Ector \<circ> \<eta>) EVrs \<rho> \<union> IImsupp' (Ector \<circ> \<eta>') EVrs \<rho>'"
 abbreviation "small_support \<delta> \<rho> \<rho>' \<equiv>
@@ -361,9 +341,453 @@ lemma Eperm_Esub:
   apply (auto simp add: fun_eq_iff Int_Un_distrib permute_\<rho> permute_\<rho>' imsupp_commute)
   done
 
-interpretation codata: Expression_with_Subst_Strong Eperm EVrs "card_suc Gbd" Ector Esub
-  by standard (auto simp: Esub_Ector\<eta> Esub_Ector\<eta>' Esub_Ector EVrs_Esub Eperm_Esub)
 
-print_statement codata.E_pbmv_axioms
+
+(**************) 
+(* That binder codatatypes satisfy the 
+strong expression axiomatization was already proved 
+in theory Codata_Customization: *)
+
+interpretation Expression_with_Surj_and_Coinduct Eperm EVrs "card_suc Gbd" Ector
+using Expression_with_Surj_and_Coinduct_axioms .
+
+
+
+(****************)
+(* Starting to prove that binder datatypes validate 
+the birecursion principle: *)
+
+
+context 
+fixes Pvalid :: "'p \<Rightarrow> bool" 
+and Pperm :: "('a::covar_G \<Rightarrow> 'a) \<Rightarrow> 'p \<Rightarrow> 'p" 
+and PVrs :: "'p \<Rightarrow> 'a set" and 
+Ector' :: "('a, 'a, 'p \<Rightarrow> 'a E, 'p \<Rightarrow> 'a E) G \<Rightarrow> 'p \<Rightarrow> 'a E"
+assumes bimodel: "Bimodel Pvalid Pperm PVrs Eperm EVrs Gbd Ector Ector'"
+begin 
+
+(* Just getting all the Bomodel theorems *)
+interpretation Bimodel Pvalid Pperm PVrs Eperm EVrs Gbd Ector Ector'
+using bimodel .
+
+(* HERE1 *)
+
+definition Evalid' :: "'a E\<times>'p \<Rightarrow> bool" where 
+"Evalid' ep \<equiv> Pvalid (snd ep)"  
+
+fun Edtor1' :: "'a E\<times>'p \<Rightarrow> (('a::covar_G,'a,'a E\<times>'p,'a E\<times>'p)G) set" where 
+"Edtor1' (e,p) =
+\<Union> { {u1 . Ector (Gmap fst fst u1) = Ector' u p \<and> 
+          GSupp1 (Gmap snd snd u1) \<union>  GSupp2 (Gmap snd snd u1) \<subseteq> {p} \<and> 
+          GVrs2 u1 \<inter> PVrs p = {} \<and> GVrs2 u1 \<inter> GVrs1 u1 = {}} | 
+       u . \<not> base u \<and> Ector (Gmap (\<lambda>pe. pe p) (\<lambda>pe. pe p) u) = e \<and> 
+           GVrs2 u \<inter> PVrs p = {} \<and> GVrs2 u \<inter> GVrs1 u = {}}"
+declare Edtor1'.simps[simp del]
+lemmas Edtor1'_def = Edtor1'.simps
+
+lemma in_Edtor1'_Ector_aux: 
+assumes "\<not> base u" "Pvalid p" "GVrs2 u \<inter> PVrs p = {}" "GVrs2 u \<inter> GVrs1 u = {}"
+shows "u1 \<in> Edtor1' (Ector (Gmap (\<lambda>pe. pe p) (\<lambda>pe. pe p) u),p) \<longleftrightarrow> 
+  (Ector (Gmap fst fst u1) = Ector' u p \<and> 
+   GSupp1 (Gmap snd snd u1) \<union> GSupp2 (Gmap snd snd u1) \<subseteq> {p} \<and> 
+   GVrs2 u1 \<inter> PVrs p = {} \<and> GVrs2 u1 \<inter> GVrs1 u1 = {})"
+using assms unfolding Edtor1'_def by (auto intro: Ector_Ector'_inj_step)
+
+lemma in_Edtor1'_Ector: 
+assumes "\<not> base u" "Pvalid p" "GVrs2 u \<inter> PVrs p = {}" "GVrs2 u \<inter> GVrs1 u = {}"
+shows "u1 \<in> Edtor1' (Ector u,p) \<longleftrightarrow> 
+  (Ector (Gmap fst fst u1) = Ector' (Gmap (\<lambda>e p. e) (\<lambda>e p. e) u) p \<and> 
+   GSupp1 (Gmap snd snd u1) \<union> GSupp2 (Gmap snd snd u1) \<subseteq> {p} \<and> 
+   GVrs2 u1 \<inter> PVrs p = {} \<and> GVrs2 u1 \<inter> GVrs1 u1 = {})"
+proof-
+  define v where v: "v \<equiv> Gmap (\<lambda>e (p::'p). e) (\<lambda>e (p::'p). e) u"
+  have u: "u = Gmap (\<lambda>pe. pe p) (\<lambda>pe. pe p) v"
+  unfolding v Gmap_comp o_def by simp
+  show ?thesis using assms apply(subst u)  
+  by (auto simp add: GVrs1_Gmap GVrs2_Gmap base_Gmap in_Edtor1'_Ector_aux v) 
+qed
+
+lemma Edtor1'_Ector: 
+assumes "\<not> base u" "Pvalid p" "GVrs2 u \<inter> PVrs p = {}" "GVrs2 u \<inter> GVrs1 u = {}" 
+shows "Edtor1' (Ector u,p) = 
+  {u1 . Ector (Gmap fst fst u1) = Ector' (Gmap (\<lambda>e p. e) (\<lambda>e p. e) u) p \<and> 
+        GSupp1 (Gmap snd snd u1) \<union> GSupp2 (Gmap snd snd u1) \<subseteq> {p} \<and> 
+        GVrs2 u1 \<inter> PVrs p = {} \<and> GVrs2 u1 \<inter> GVrs1 u1 = {}}"
+using in_Edtor1'_Ector[OF assms] by auto
+
+fun Edtor' :: "'a E\<times>'p \<Rightarrow> 'a E + (('a::covar_G,'a,'a E\<times>'p,'a E\<times>'p)G)set" where 
+"Edtor' (e,p) = (let u = (SOME u. e = Ector u) in 
+  if base u then Inl (Ector' (Gmap (\<lambda>a p. a) (\<lambda>a p. a) u) p) else Inr (Edtor1' (e,p)))"
+declare Edtor'.simps[simp del]
+lemmas Edtor'_def = Edtor'.simps
+
+lemma Edtor'_base: 
+assumes "base u"
+shows "Edtor' (Ector u, p) = Inl (Ector' (Gmap (\<lambda>a p. a) (\<lambda>a p. a) u) p)"
+using assms unfolding Edtor'_def 
+by (smt (verit, ccfv_threshold) Eps_cong base_Some_Ector)
+
+
+lemma Edtor'_step: 
+assumes "\<not> base u"
+shows "Edtor' (Ector u, p) = Inr (Edtor1' (Ector u, p))"
+using assms unfolding Edtor'_def 
+by (smt (verit) Ector_base tfl_some) 
+
+lemma Edtor'_Inl_base: "Edtor' (Ector u, p) = Inl U \<Longrightarrow> base u"
+  using Edtor'_step by force 
+
+lemma Edtor'_Inr_step: "Edtor' (Ector u, p) = Inr U \<Longrightarrow> \<not> base u"
+  using Edtor'_base by force
+
+find_theorems Ector name: surj
+
+
+(* *)
+lemma Edtor1'_NE: 
+assumes base: "\<not> base u" and p: "Pvalid p"
+shows "Edtor1' (Ector u, p) \<noteq> {}" using in_Edtor1'_Ector
+proof-
+  obtain u0 where u0u: "Ector u0 = Ector u" 
+  and g: "GVrs2 u0 \<inter> PVrs p = {}" "GVrs2 u0 \<inter> GVrs1 u0 = {}" 
+  using Ector_fresh_surj'[OF PVrs_small, OF p] by metis
+  hence base: "\<not> base u0" using base using Ector_base by blast
+  obtain uu1 where "Ector uu1 = Ector' (Gmap (\<lambda>e p. e) (\<lambda>e p. e) u0) p" 
+  "GVrs2 uu1 \<inter> PVrs p = {}" "GVrs2 uu1 \<inter> GVrs1 uu1 = {}"
+  using Ector_fresh_surj'[OF PVrs_small, OF p] by metis
+  then have "Gmap (\<lambda>e. (e,p)) (\<lambda>e. (e,p)) uu1 \<in> Edtor1' (Ector u, p)" 
+  unfolding u0u[symmetric] apply(subst in_Edtor1'_Ector[OF base p g]) apply safe
+    subgoal unfolding Gmap_comp o_def by simp
+    subgoal unfolding GSupp1_Gmap by auto
+    subgoal unfolding GSupp2_Gmap by auto
+    subgoal unfolding GVrs2_Gmap by auto 
+    subgoal unfolding GVrs1_Gmap GVrs2_Gmap by auto .
+  thus ?thesis by auto
+qed
+
+
+lemma Udtor_ne: "Evalid' d \<Longrightarrow> Edtor' d = Inr X \<Longrightarrow> X \<noteq> {}"
+apply (cases d) apply safe 
+  subgoal for e p apply(rule Ector_exhaust'[of e]) apply simp
+  subgoal for u apply(cases "base u")
+    subgoal unfolding Edtor'_base by simp
+    subgoal unfolding Edtor'_step Evalid'_def using Edtor1'_NE by simp . . .
+
+fun EVrs'' where "EVrs'' (e,p) = EVrs e \<union> PVrs p"
+declare EVrs''.simps[simp del]
+lemmas EVrs''_def = EVrs''.simps
+
+fun Eperm'' where "Eperm'' \<sigma> (e,p) = (Eperm \<sigma> e, Pperm \<sigma> p)"
+declare Eperm''.simps[simp del]
+lemmas Eperm''_def = Eperm''.simps
+
+lemma fst_EPerm'[simp]: "fst \<circ> Eperm'' \<sigma> = Eperm \<sigma> o fst"
+unfolding fun_eq_iff by (simp add: Eperm''_def)
+
+lemma snd_EPerm'[simp]: "snd \<circ> Eperm'' \<sigma> = Pperm \<sigma> o snd"
+unfolding fun_eq_iff by (simp add: Eperm''_def)
+
+lemma Eperm''_id[simp]: "Pvalid (snd pe) \<Longrightarrow> Eperm'' id pe = pe"
+  using Eperm''_def  
+  by (metis Eperm_id Pperm_id id_apply snd_conv surj_pair)   
+
+abbreviation small :: "('a::covar_G \<Rightarrow>'a) \<Rightarrow> bool"  
+where "small \<sigma> \<equiv> |supp \<sigma>| <o |UNIV::'a set|"
+
+lemma Eperm''_o: 
+"Pvalid (snd ep) \<Longrightarrow> small \<sigma>1 \<Longrightarrow> bij \<sigma>1 \<Longrightarrow> small \<sigma>2 \<Longrightarrow> bij \<sigma>2 \<Longrightarrow> 
+Eperm'' (\<sigma>1 \<circ> \<sigma>2) ep = Eperm'' \<sigma>1 (Eperm'' \<sigma>2 ep)"
+apply(cases ep) 
+by (simp add: Eperm''_def Eperm_comp Pperm_comp Eperm_comp') 
+
+lemma Eperm''_comp: 
+"Pvalid p \<Longrightarrow> small \<sigma>1 \<Longrightarrow> bij \<sigma>1 \<Longrightarrow> small \<sigma>2 \<Longrightarrow> bij \<sigma>2 \<Longrightarrow> 
+ Eperm'' \<sigma>1 (Eperm'' \<sigma>2 (e,p)) = Eperm'' (\<sigma>1 \<circ> \<sigma>2) (e,p)"
+by (simp add: Eperm''_def Eperm_comp Pperm_comp Eperm_comp') 
+
+lemma Eperm''_cong:
+"Pvalid p \<Longrightarrow> small \<sigma>1 \<Longrightarrow> bij \<sigma>1 \<Longrightarrow>
+ small \<sigma>2 \<Longrightarrow> bij \<sigma>2 \<Longrightarrow> \<forall>a\<in>EVrs'' (e,p). \<sigma>1 a = \<sigma>2 a \<Longrightarrow> Eperm'' \<sigma>1 (e,p) = Eperm'' \<sigma>2 (e,p)"
+unfolding Eperm''_def EVrs''_def    
+by (metis Eperm_cong Pperm_cong UnCI)    
+
+(* HERE *)
+term term 
+(* 
+lemma nomC: "nom Evalid' Eperm'' EVrs''"
+unfolding nom_def apply safe
+ unfolding Evalid'_def Eperm''_def using nomP unfolding nom_def apply simp  
+apply auto  
+  apply (auto simp add: EVrs''_def Eperm_comp Pperm_comp)
+  apply (metis Eperm_cong Un_iff) 
+  by (metis Pperm_cong Un_iff) 
+
+lemma Pvalid_Pperm[simp]: "Pvalid p \<Longrightarrow> small \<sigma> \<Longrightarrow> bij \<sigma> \<Longrightarrow> Pvalid (Pperm \<sigma> p)"
+using nomP unfolding nom_def by blast
+
+lemma dtorPermC: "dtorPermC Evalid' Edtor' Eperm''"
+unfolding dtorPermC_def apply clarify subgoal for \<sigma> e p
+unfolding Eperm''_def Evalid'_def 
+  apply(rule Ector_exhaust_fresh[OF "countable_PVrs_im", of \<sigma> p e], simp_all)
+  unfolding A_Int_Un_emp apply(erule conjE) apply simp
+  subgoal for u apply(cases "base u")
+    subgoal unfolding Edtor'_base apply safe 
+    unfolding Eperm_Ector apply(subst Edtor'_base)
+      subgoal using base_Gmap base_Gren by metis
+      subgoal apply auto 
+      apply(subst ctorPermM_Ector'[unfolded ctorPermM_def, rule_format])
+        subgoal by simp
+        subgoal unfolding Gmap_comp Gmap_Gren unfolding lift_def o_def .. . .
+     subgoal 
+     apply(subgoal_tac "\<sigma> ` GVrs2 u \<inter> PVrs p = {}") 
+     prefer 2 subgoal unfolding bij_inv_Un_triv by auto
+     unfolding Edtor'_step apply safe 
+     unfolding Eperm_Ector apply(subst Edtor'_step)
+      subgoal using base_Gmap base_Gren by metis
+      subgoal apply simp  
+      apply(subst Edtor1'_Ector)
+        subgoal using base_Gmap base_Gren by metis
+        subgoal by auto
+        subgoal unfolding GVrs2_Gmap GVrs2_Gren PVrs_Pperm  
+          by (metis bij_is_inj image_Int image_empty)
+        subgoal unfolding GVrs2_Gmap GVrs2_Gren GVrs1_Gmap GVrs1_Gren PVrs_Pperm  
+        by (simp add: image_Int_empty) 
+        subgoal unfolding image_def apply auto apply(subst Edtor1'_Ector)
+        apply auto subgoal for u0
+        apply(rule exI[of _ "Gren (inv \<sigma>) (inv \<sigma>) u0"]) apply safe
+          prefer 2 subgoal apply(subst Gren_comp) by auto
+          subgoal 
+          apply(rule exI[of _ "Gren (inv \<sigma>) (inv \<sigma>) (Gmap (Eperm'' (inv \<sigma>)) (Eperm'' (inv \<sigma>)) u0)"])
+          apply safe
+            subgoal unfolding Gmap_comp Gmap_Gren apply(subst Gmap_Gren)
+              subgoal by auto
+              subgoal by auto
+              subgoal unfolding Gmap_comp apply simp 
+              unfolding Gmap_o apply(subst o_def)
+              apply(subst Eperm_Ector[symmetric])
+                subgoal by auto
+                subgoal by auto
+                subgoal 
+                unfolding Gmap_o[symmetric] triv_Eperm_lift unfolding Gmap_o
+                unfolding o_def
+                apply(subst (asm) ctorPermM_Ector'[unfolded ctorPermM_def, rule_format,  
+                            symmetric]) 
+                  subgoal by simp
+                  subgoal apply(subst Eperm_inv_iff) by auto . . .
+              subgoal for e' unfolding GSupp1_Gmap apply auto subgoal for b apply(subst (asm) GSupp1_Gren)
+                subgoal by auto
+                subgoal by auto
+                subgoal unfolding GSupp1_Gmap apply(auto simp: Eperm''_def) subgoal for ee pp 
+                apply(subgoal_tac "pp = Pperm \<sigma> p")
+                  subgoal apply simp apply(subst Pperm_comp) by auto
+                  subgoal by auto . . . .
+              subgoal for pp unfolding GSupp2_Gmap apply auto apply(subst (asm) GSupp2_Gren)
+                subgoal by auto
+                subgoal by auto
+                subgoal for ee unfolding GSupp2_Gmap apply(auto simp: Eperm''_def) subgoal for e' p'
+                apply(subgoal_tac "p' = Pperm \<sigma> p")
+                  subgoal apply simp apply(subst Pperm_comp) by auto
+                  subgoal by auto . . . 
+              subgoal for a apply(subst (asm) GVrs2_Gren)
+                subgoal by auto subgoal by auto
+                subgoal unfolding GVrs2_Gmap GSupp1_Gmap GSupp2_Gmap apply auto  
+                subgoal for a
+                apply(subgoal_tac "a \<in> \<sigma> ` PVrs p") 
+                  subgoal by (metis IntI PVrs_Pperm empty_iff)
+                  subgoal unfolding bij_in_inv_Un_triv . . . .
+              subgoal by (metis (no_types, lifting) GVrs1_Gmap GVrs1_Gren GVrs2_Gmap 
+                    GVrs2_Gren bij_betw_inv_into bij_in_inv_Un_triv disjoint_iff small_inv)
+              subgoal apply(subst Gmap_Gren[symmetric])
+               subgoal by auto subgoal by auto
+               subgoal unfolding Gmap_comp  
+               apply(rule sym) apply(rule Gmap_cong_id)
+                 subgoal for ea unfolding o_def
+                 apply(subst Eperm''_o[symmetric]) apply (cases ea) apply auto 
+                 subgoal  
+                   by (metis (no_types, opaque_lifting) GSupp1_Gmap GSupp1_Gren Pvalid_Pperm
+                       bij_betw_inv_into insert_image insert_subset singletonD small_inv snd_conv) 
+                 apply(subst (asm) GSupp1_Gren) 
+                 by (auto simp: GSupp1_Gmap subset_iff) 
+                 subgoal for ea unfolding o_def
+                 apply(subst Eperm''_o[symmetric]) apply (cases ea)  apply auto 
+                 apply(subst (asm) GSupp2_Gren) apply (auto simp: GSupp2_Gmap subset_iff)
+                 by (metis (no_types, opaque_lifting) Eperm''_id GSupp2_Gren Pvalid_Pperm
+                     bij_betw_inv_into imageI small_inv)
+ . . . . . . . . . .
+               
+
+lemma dtorVrsGrenC: "dtorVrsGrenC Evalid' Edtor' Eperm'' EVrs''"
+unfolding dtorVrsGrenC_def EVrs''_def proof safe 
+  fix e p U u1 u2 
+  assume "Evalid' (e, p)"
+  and 0: "Edtor' (e, p) = Inr U" and u12: "{u1, u2} \<subseteq> U"
+  hence P: "Pvalid p" unfolding Evalid'_def by simp
+  show "\<exists>\<sigma>. small \<sigma> \<and>
+           bij \<sigma> \<and>
+           id_on ((\<Union> (EVrs'' ` GSupp1 u1) - GVrs2 u1)) \<sigma> \<and>
+           Gren id \<sigma> (Gmap (Eperm'' \<sigma>) id u1) = u2"
+  proof(rule Ector_exhaust_fresh[OF countable_PVrs, of p e, OF P])
+    fix u assume e: "e = Ector u" and g: "GVrs2 u \<inter> PVrs p = {}" "GVrs2 u \<inter> GVrs1 u = {}"
+    show ?thesis proof(cases "base u")
+      case True
+      show ?thesis using 0 unfolding e Edtor'_base[OF True] by simp
+    next
+      case False
+      hence U: "Edtor1' (Ector u, p) = U" using 0 unfolding e Edtor'_step[OF False] by simp
+      hence U: "U =
+      {u1. Ector (Gmap fst fst u1) = Ector' (Gmap (\<lambda>e p. e) (\<lambda>e p. e) u) p \<and>
+           GSupp1 (Gmap snd snd u1) \<subseteq> {p} \<and> GSupp2 (Gmap snd snd u1) \<subseteq> {p} \<and> 
+           GVrs2 u1 \<inter> PVrs p = {} \<and> GVrs2 u1 \<inter> GVrs1 u1 = {}}"  
+      unfolding Edtor1'_Ector[OF False P g] by auto
+
+      hence u1: "Ector (Gmap fst fst u1) = Ector' (Gmap (\<lambda>e p. e) (\<lambda>e p. e) u) p"
+           "GSupp1 (Gmap snd snd u1) \<subseteq> {p}" "GSupp2 (Gmap snd snd u1) \<subseteq> {p}" "GVrs2 u1 \<inter> PVrs p = {}"
+      and u2: "Ector (Gmap fst fst u2) = Ector' (Gmap (\<lambda>e p. e) (\<lambda>e p. e) u) p"
+          "GSupp1 (Gmap snd snd u2) \<subseteq> {p}" "GSupp2 (Gmap snd snd u2) \<subseteq> {p}" "GVrs2 u2 \<inter> PVrs p = {}"
+      using u12 by auto
+
+      have 00: "PVrs p \<inter> GVrs2 (Gmap fst fst u1) = {}" using u1 by (auto simp: GVrs2_Gmap)
+      note eq = u1(1)[unfolded u2(1)[symmetric]]
+      
+      obtain \<sigma> where ss: "bij \<sigma> \<and> small \<sigma>"
+        "id_on 
+         ((\<Union> (EVrs ` GSupp1 (Gmap fst fst u1)) - GVrs2 (Gmap fst fst u1)) \<union> PVrs p )
+         \<sigma>"
+        "Gren id \<sigma> (Gmap (Eperm \<sigma>) id (Gmap fst fst u1)) = Gmap fst fst u2"   
+        using Ector_eq_imp_strong[of "Gmap fst fst u1" "Gmap fst fst u2", OF eq countable_PVrs 00, OF P]
+        by blast
+      have io: "\<And>e' p' a. (e',p') \<in> GSupp1 u1 \<Longrightarrow> a \<in> EVrs e' \<Longrightarrow> a \<notin> GVrs2 u1 \<Longrightarrow> \<sigma> a = a"
+          "\<And>a. a \<in> PVrs p \<Longrightarrow> \<sigma> a = a" 
+      using ss(2) unfolding id_on_def by (fastforce simp: GSupp1_Gmap GSupp2_Gmap GVrs2_Gmap)+
+
+      show ?thesis proof(rule exI[of _ \<sigma>], safe)
+        show "small \<sigma>" "bij \<sigma>" using ss by auto
+      next
+        show "id_on ((\<Union> (EVrs'' ` GSupp1 u1) - GVrs2 u1)) \<sigma>"
+        unfolding id_on_def image_def proof(auto simp: EVrs''_def)
+          fix a e' p' assume "(e', p') \<in> GSupp1 u1" "a \<in> EVrs e'" "a \<notin> GVrs2 u1" 
+          thus "\<sigma> a = a" using io(1) by auto
+        next
+          fix a e' p' assume aa: "(e', p') \<in> GSupp1 u1" "a \<in> PVrs p'"  "a \<notin> GVrs2 u1"
+          hence "p' = p" using u1(2) unfolding GSupp1_Gmap by auto  
+          thus "\<sigma> a = a" using aa io(2) by auto
+        qed
+      next
+        have ss3: "Gmap (Eperm \<sigma>) id (Gmap fst fst (Gren id \<sigma> u1)) = Gmap fst fst u2"
+        unfolding ss(3)[symmetric] 
+        by (simp add: Gmap_Gren ss(1)) 
+
+        have gg: "Gmap (Eperm'' \<sigma>) id (Gren id \<sigma> u1) = u2"
+        apply(subst snd_single_Gmap'[symmetric, where t = u2 and p = p])
+          subgoal by (metis GSupp1_Gmap u2(2))
+          subgoal by (metis GSupp2_Gmap u2(3))
+          subgoal apply(subst snd_single_Gmap'[symmetric, where t = "Gren id \<sigma> u1" and p = p])
+            subgoal by (metis GSupp1_Gmap GSupp1_Gren bij_id small_id ss(1) u1(2))
+            subgoal by (metis GSupp2_Gmap GSupp2_Gren bij_id small_id ss(1) u1(3))
+            subgoal unfolding ss3[symmetric] unfolding Gmap_comp unfolding o_def Eperm''_def
+            apply(rule Gmap_cong)
+              subgoal by (metis P Pperm_cong Pperm_id bij_id eq_id_iff io(2) small_id ss(1))
+              subgoal by simp . . .
+        show "Gren id \<sigma> (Gmap (Eperm'' \<sigma>) id u1) = u2"
+        unfolding gg[symmetric]  
+        by (simp add: Gmap_Gren ss(1)) 
+      qed
+    qed
+  qed
+qed
+
+lemma step_Ector'_Ector_EVrs: 
+"\<not> base u \<Longrightarrow> Pvalid p \<Longrightarrow> EVrs'' (Ector' (Gmap (\<lambda>e p. e) (\<lambda>e p. e) u) p, p) \<subseteq> PVrs p \<union> EVrs (Ector u)"
+unfolding EVrs''_def apply(rule tri_Un1) 
+apply(rule subset_trans[OF ctorVarsM_Ector'[unfolded ctorVarsM_def, rule_format]])
+  subgoal .
+  subgoal apply(rule tri_Un3) unfolding EVrs_Ector GSupp1_Gmap GVrs1_Gmap apply auto  
+    apply (metis Diff_iff GVrs2_Gmap)  
+    by (metis GSupp2_Gmap image_iff) .
+
+lemma base_Ector'_Ector_EVrs: 
+"base u \<Longrightarrow> Pvalid p \<Longrightarrow> EVrs'' (Ector' (Gmap (\<lambda>e p. e) (\<lambda>e p. e) u) p, p) \<subseteq> PVrs p \<union> EVrs (Ector u)"
+unfolding EVrs''_def apply(rule tri_Un1) 
+apply(rule subset_trans[OF ctorVarsM_Ector'[unfolded ctorVarsM_def, rule_format]])
+  subgoal .
+  subgoal apply(rule tri_Un3) unfolding EVrs_Ector GSupp1_Gmap GVrs1_Gmap apply auto 
+  apply (simp add: base_base) 
+    by (simp add: base_Gmap base_base) .
+
+lemma dtorVrsC: "dtorVrsC Evalid' Edtor' EVrs''"
+unfolding EVrs''_def
+unfolding dtorVrsC_def Evalid'_def apply (intro allI impI) subgoal for pe apply(cases pe) subgoal for e p 
+apply clarsimp
+apply(rule Ector_exhaust_fresh[OF countable_PVrs, of p e]) apply clarify apply (intro conjI allI)
+  subgoal for u apply(cases "base u")
+    subgoal unfolding Edtor'_base using Edtor'_Inr_step by auto
+    subgoal apply clarify unfolding Edtor'_step  
+    unfolding Edtor1'_Ector unfolding EVrs_Ector GSupp1_Gmap GSupp2_Gmap apply clarify
+    subgoal for ua  
+    apply(rule incl_Un_triv3)
+    unfolding EVrs''_def EVrs_Ector 
+    apply(rule subset_trans[OF _ Ector_Ector'_EVrs_step'[of p "Gmap fst fst ua", unfolded GSupp1_Gmap 
+      GSupp2_Gmap GVrs1_Gmap GVrs2_Gmap]]) 
+      subgoal apply(rule incl_Un3_triv3)
+        subgoal ..
+        subgoal by auto (metis (lifting) DiffI fst_conv image_eqI)   
+        subgoal by auto fastforce .
+      subgoal .
+      subgoal .
+    subgoal using Edtor'_step in_Edtor1'_Ector by auto . . .
+  subgoal for u apply(cases "base u")
+    subgoal using base_Ector'_Ector_EVrs unfolding Edtor'_base EVrs''_def 
+      by (metis Edtor'_base Un_commute Un_subset_iff old.sum.inject(1))
+    subgoal unfolding Edtor'_step using Edtor'_Inl_base by blast . . . .
+
+
+lemma presDV_Evalid'_Edtor': "presDV Evalid' Edtor'"
+unfolding presDV_def apply clarify
+  subgoal for e p U u' e' p'
+  unfolding Evalid'_def snd_conv apply(rule Ector_exhaust_fresh[OF countable_PVrs, of p e])
+    subgoal .
+    subgoal for u apply(cases "base u")
+      subgoal apply clarify unfolding Edtor'_base by auto
+      subgoal apply clarify unfolding Edtor'_step Edtor1'_Ector 
+      by (auto simp: GSupp1_Gmap GSupp2_Gmap) . . .
+       
+lemma presPV_Evalid'_Eperm'': "presPV Evalid' Eperm''"
+unfolding presPV_def apply clarify subgoal for \<sigma> e p 
+unfolding Eperm''_def Evalid'_def by simp .
+
+
+
+
+(* HERE2 *)
+
+
+
+end (* context *)
+
+
+(**************) 
+(* Binder codatatypes validate the 
+birecursion principle: *)
+
+interpretation Expression_with_Birecursor Eperm EVrs "card_suc Gbd" Ector
+proof (standard, safe)
+  fix Pvalid :: "'p \<Rightarrow> bool"
+  and Pperm :: "('a \<Rightarrow> 'a) \<Rightarrow> 'p \<Rightarrow> 'p"
+  and PVrs :: "'p \<Rightarrow> 'a set"
+  and Ector' :: "('a, 'a, 'p \<Rightarrow> 'a E, 'p \<Rightarrow> 'a E) G \<Rightarrow> 'p \<Rightarrow> 'a E"
+  assume "Bimodel Pvalid Pperm PVrs Eperm EVrs (card_suc Gbd) Ector Ector'"
+  (* interpret corec: COREC  *)
+  (* term corec.COREC *)
+  show "\<exists>rec. (\<forall>u p. Pvalid p \<and> noclashE u \<and> GVrs2 u \<inter> PVrs p = {} \<longrightarrow> 
+    rec (Ector u) p = Ector' (Gmap rec rec u) p) \<and>
+    (\<forall>e p \<sigma>. bij \<sigma> \<longrightarrow> |supp \<sigma>| <o |UNIV| \<longrightarrow> Pvalid p \<longrightarrow> rec (Eperm \<sigma> e) p = Eperm \<sigma> (rec e (Pperm (inv \<sigma>) p))) \<and>
+    (\<forall>e p. Pvalid p \<longrightarrow> EVrs (rec e p) \<subseteq> PVrs p \<union> EVrs e)"
+    sorry
+qed
+
+interpretation birec_codata: Expression_with_Birecursor_for_Subst_Strong Eperm EVrs "card_suc Gbd" Ector
+  by standard
+
+print_statement birec_codata.Esub_Strong.E_pbmv_axioms
 
 end
